Otway-Rees: proved "no (mutual) auth" for msg 1 interception and responder impersonation attacks
In both attacks, the actual responder is not involved in the protocol runs.
However, the initiator believes it is talking to the actual responder and not
to the attacker or a principal corrupted by the attacker. --> No auth at all.

otway-rees/OYRS.Attacker.fst
@@ -284,4 +284,23 @@ let attacker_knows_conv_key_stored_in_initiator_or_responder_state
     if k_ab = conv_key then () else error "attacker could not derive conversation key\n"
   | Success (S.InitiatorRecvedMsg4 srv b k_ab) ->
     if k_ab = conv_key then () else error "attacker could not derive conversation key\n"
-  | _ -> ()
+  | _ -> error "not a final principal state\n"
+
+val initiator_believes_responder_authenticated:
+  i:principal ->
+  si:nat ->
+  r:principal ->
+  LCrypto unit (L.pki S.oyrs_preds)
+  (requires (fun t0 -> True))
+  (ensures (fun t0 _ t1 -> True))
+
+let initiator_believes_responder_authenticated
+  i
+  si
+  r
+= let now = global_timestamp () in
+  let (|_,ser_st|) = L.get_session #(S.oyrs_preds) #now i si in
+  match S.parse_session_st ser_st with
+  | Success (S.InitiatorRecvedMsg4 srv b k_ab) ->
+    if b = r then () else error "initiator does not believe to talk to responder\n"
+  | _ -> error "wrong state\n"
